fix remaining bug in handler and update proof,
now the only two inline admits in softmul_correct are about
nextPc = pc+4 (which only holds at the end of each instruction,
but not in the middle of executing an instruction), and thus
will need careful invariant crafting.
Still inline admits in SoftmulCompile and many toplevel axioms.

compiler/src/compilerExamples/Softmul.v
@@ -121,12 +121,13 @@ Section WithRegisterNames.
   Remark MScratch_correct: CSR.lookupCSR MScratch = CSR.MScratch. reflexivity. Qed.
 
   Definition handler_init := [[
-    Csrrw sp sp MScratch;
-    Addi sp sp (-128); (* amount of stack we need to save the 32 registers *)
-    Sw sp zero 0;
-    Sw sp ra 4;
-    Csrr ra MScratch;
-    Sw sp ra 8
+    Csrrw sp sp MScratch;  (* swap sp and MScratch CSR *)
+    Sw sp zero (-128);     (* save the 0 register (for uniformity) *)
+    Sw sp ra (-124);       (* save ra *)
+    Csrr ra MScratch;      (* use ra as a temporary register... *)
+    Sw sp ra (-120);       (* ... to save the original sp *)
+    Csrw sp MScratch;      (* restore the original value of MScratch *)
+    Addi sp sp (-128)      (* remainder of code will be relative to updated sp *)
   ]].
 
   Definition inc_mepc := [[
@@ -147,9 +148,11 @@ Section WithRegisterNames.
     Jal ra (Z.of_nat (1 + List.length inc_mepc + 29 + List.length handler_final) * 4)
   ]].
 
-  Definition handler_insts :=
+  Definition asm_handler_insts :=
     handler_init ++ save_regs3to31 ++ call_mul ++ inc_mepc ++
-       restore_regs3to31 ++ handler_final ++ mul_insts.
+       restore_regs3to31 ++ handler_final.
+
+  Definition handler_insts := asm_handler_insts ++ mul_insts.
 End WithRegisterNames.
 
 Section Riscv.
@@ -164,6 +167,11 @@ Section Riscv.
   Local Notation M := (free riscv_primitive primitive_result).
 
   Local Hint Mode map.map - - : typeclass_instances.
+
+  Lemma truncated_scalar_unique: forall [addr z m],
+      (addr |-> truncated_scalar access_size.four z) m ->
+      eq m = (addr |-> truncated_scalar access_size.four z).
+  Admitted.
 
   Declare Scope array_abbrevs_scope.
   Open Scope array_abbrevs_scope.
@@ -680,11 +688,13 @@ Section Riscv.
       end
     | |- _ => compareZconsts
     | |- map.get _ _ = Some _ => eassumption
-    | |- map.get _ _ <> None => congruence
+    | |- _ <> None => congruence
     | |- map.get (map.set _ _ _) _ = _ => unfold map.set
     | |- map.get (map.put _ ?x _) ?x = _ => eapply map.get_put_same
     | |- map.get (map.put _ _ _) _ = _ => eapply get_put_diff_eq_l; [compareZconsts|]
-    | |- map.get (map.put _ ?x _) ?x <> None => rewrite map.get_put_same; clear; congruence
+    | |- map.get (map.set _ _ _) _ <> None => unfold map.set
+    | |- map.get (map.put _ ?x _) ?x <> None => rewrite map.get_put_same
+    | |- map.get (map.put _ ?x _) ?y <> None => rewrite map.get_put_diff by congruence
     | |- regs_initialized (map.put _ _ _) => eapply preserve_regs_initialized_after_put
     | |- regs_initialized (map.set _ _ _) => eapply preserve_regs_initialized_after_put
     | |- mcomp_sat endCycleNormal _ _ => eapply mcomp_sat_endCycleNormal
@@ -908,19 +918,22 @@ Section Riscv.
       (* Csrrw sp sp MScratch *)
       eapply runsToStep_cps. repeat step.
 
-      (* Addi sp sp (-128) *)
+      (* Sw sp zero (-128) *)
       eapply runsToStep_cps. repeat step.
 
-      (* Sw sp zero 0        (needed if the instruction to be emulated reads register 0) *)
-      eapply runsToStep_cps. repeat step.
-
-      (* Sw sp ra 4 *)
+      (* Sw sp ra (-124) *)
       eapply runsToStep_cps. repeat step.
 
       (* Csrr ra MScratch *)
       eapply runsToStep_cps. repeat step.
 
-      (* Sw sp ra 8 *)
+      (* Sw sp ra (-120) *)
+      eapply runsToStep_cps. repeat step.
+
+      (* Csrw sp MScratch *)
+      eapply runsToStep_cps. repeat step.
+
+      (* Addi sp sp (-128) *)
       eapply runsToStep_cps. repeat step.
 
       (* save_regs3to31 *)
@@ -930,7 +943,7 @@ Section Riscv.
       { repeat step. }
       autorewrite with rew_word_morphism. repeat word_simpl_step_in_goal.
 
-      unfold handler_insts in ML.
+      unfold handler_insts, asm_handler_insts in ML.
       rewrite !(array_app (E := Instruction)) in ML.
       repeat match type of ML with
              | context[List.length ?l] => let n := concrete_list_length l in
@@ -1100,10 +1113,6 @@ Section Riscv.
         - erewrite nth_error_nth' by lia. reflexivity.
       }
 
-      match goal with
-      | H: _ |- _ => rewrite map.get_put_diff in H by
-            (unfold RegisterNames.sp, RegisterNames.ra; lia)
-      end.
       replace (nth (Z.to_nat rs1) (word.of_Z 0 :: v0 :: v :: vals) default) with
               (getReg (regs initialH) rs1) in *.
       2: {
@@ -1310,26 +1319,10 @@ Section Riscv.
                                       (Z.to_nat rd)
                                       (word.mul (getReg (regs initialH) rs1)
                                          (getReg (regs initialH) rs2)))).
-
-Set Nested Proofs Allowed.
-
-  Lemma subst_split_bw: forall (m m1 m2 M : Mem) (R : Mem -> Prop),
-      map.split m m1 m2 ->
-      sep (sep (eq m1) (eq m2)) R M ->
-      sep (eq m) R M.
-  Proof.
-    unfold sep, map.split. intros. fwd. eauto 10.
-  Qed.
-
-  Lemma truncated_scalar_unique: forall [addr z m],
-      (addr |-> truncated_scalar access_size.four z) m ->
-      eq m = (addr |-> truncated_scalar access_size.four z).
-  Admitted.
-
           cbn [seps]. eapply subst_split_bw. 1: eassumption.
           rewrite (truncated_scalar_unique MHI).
 
-          unfold handler_insts.
+          unfold handler_insts, asm_handler_insts.
           rewrite !(array_app (E := Instruction)).
           repeat match goal with
                  | |- context[List.length ?l] => let n := concrete_list_length l in
@@ -1340,9 +1333,6 @@ Set Nested Proofs Allowed.
           replace (pc initialH) with (pc initialL) in *.
           cbn [seps] in ML. use_sep_assumption.
           cancel.
-          (* BUG: v doesn't match (word.of_Z stack_hi) because we forgot to
-             reset MScratch to its original value! *)
-          case TODO. (* separation logic *)
         }
         { listZnWords. }
       }
